[:string], [:string-byte-size-at-most n]

src/3d/ocaml/lexer.mll
@@ -125,6 +125,8 @@ rule token =
   | "[:byte-size"                { locate lexbuf LBRACK_BYTESIZE }
   | "[:byte-size-at-most"        { locate lexbuf LBRACK_BYTESIZE_AT_MOST }
   | "[:byte-size-single-element-array" { locate lexbuf LBRACK_SINGLE_ELEMENT_BYTESIZE }
+  | "[:string"     { locate lexbuf LBRACK_STRING }
+  | "[:string-byte-size-at-most"     { locate lexbuf LBRACK_STRING_AT_MOST }
   | "["                          { locate lexbuf LBRACK (* intended for use with UINT8 arrays only, interpreted as [:byte-size] *)}
   | "]"                          { locate lexbuf RBRACK }
   | "[="           { deprecation_warning lexbuf "[:byte-size-single-element-array";
